make `WeakestPrecondition.cmd` complete wrt `Semantics.exec` (#361)
* define a WP.cmd' in terms of exec, might soon replace WP.cmd

and rules for cmd' whose premises are copied from WP.cmd.
This one is "fs everywhere" (ie list of functions everywhere).
The wp_call rule requires a NoDup, which would be cumbersome to
carry around.

* dead simple `call` based on `map.get`

* convert from "fs everywhere" to "env everywhere"

* instead of unfold1_cmd_goal, eapply lemma_corresponding_to_command

In an "env everywhere" setting, where program_logic_goal_for!
adds a (map.get fs fname = Some fimpl) hypothesis.
Surprise #1: There's no case in straightline that handles if-then-else
Surprise #2: unfold1_... tactics are not the only place that depend
on conversion: There also exists a letexists in SPI that turns a
(WP (cmd.cond e _ _) ...) into an (exists v, eval e v /\ ...), and
probably more elsewhere.

* wip "env everywhere" approach

* make WeakestPrecondition.cmd complete wrt exec

by leaving the structurally recursive cases of cmd_body unchanged,
and defining the two non-structurally recursive cases (loop and call)
directly in terms of exec.
This seems to be the only approach that does not break proofs in
bedrock2Examples too badly.

* hardcode env implementation in bedrock2.Semantics,

and update compiler, LiveVerif, end2end

* add back program/Proper_program because it's used by rupicola

* cp Semantics.v MetricSemantics.v

* bedrock2.Semantics is now metrics-free, and metrics are in MetricSemantics

* refinement lemmas for induction over command syntax

* delete WP.v (opaque Module), only LAN9250 needed fixing

* LiveVerif: wp_cmd is exec instead of WeakestPrecondition.cmd

* env doesn't really need to be an Instance, it seems

* fix argument order in refinement

bedrock2/src/bedrock2/ProgramLogic.v
@@ -1,11 +1,12 @@
 From coqutil.Tactics Require Import Tactics letexists eabstract rdelta reference_to_string ident_of_string.
+Require Import coqutil.Map.Interface.
 Require Import bedrock2.Syntax.
 Require Import bedrock2.WeakestPrecondition.
 Require Import bedrock2.WeakestPreconditionProperties.
 Require Import bedrock2.Loops.
 Require Import bedrock2.Map.SeparationLogic bedrock2.Scalars.
 
-Definition spec_of (procname:String.string) := list (String.string * (list String.string * list String.string * Syntax.cmd.cmd)) -> Prop.
+Definition spec_of (procname:String.string) := Semantics.env -> Prop.
 Existing Class spec_of.
 
 Module Import Coercions.
@@ -55,9 +56,9 @@ Ltac program_logic_goal_for_function proc :=
   let __ := constr:(proc : Syntax.func) in
   constr_string_basename_of_constr_reference_cps ltac:(Tactics.head proc) ltac:(fun fname =>
   let spec := lazymatch constr:(_:spec_of fname) with ?s => s end in
-  exact (forall functions : list (string * Syntax.func), ltac:(
+  exact (forall (functions : @map.rep _ _ Semantics.env) (EnvContains : map.get functions fname = Some proc), ltac:(
     let callees := eval cbv in (callees (snd proc)) in
-    let s := assuming_correctness_of_in callees functions (spec (cons (fname, proc) functions)) in
+    let s := assuming_correctness_of_in callees functions (spec functions) in
     exact s))).
 Definition program_logic_goal_for (_ : Syntax.func) (P : Prop) := P.
 
@@ -84,7 +85,7 @@ Ltac bind_body_of_function f_ :=
 
 (* note: f might have some implicit parameters (eg a record of constants) *)
 Ltac enter f :=
-  cbv beta delta [program_logic_goal_for]; intros;
+  cbv beta delta [program_logic_goal_for];
   bind_body_of_function f;
   lazymatch goal with |- ?s ?p => let s := rdelta s in change (s p); cbv beta end.
 
@@ -229,9 +230,10 @@ Ltac straightline :=
   | _ => straightline_cleanup
   | |- program_logic_goal_for ?f _ =>
     enter f; intros;
-    unfold1_call_goal; cbv match beta delta [call_body];
-    lazymatch goal with |- if ?test then ?T else _ =>
-      replace test with true by reflexivity; change T end;
+    match goal with
+    | H: map.get ?functions ?fname = Some _ |- _ =>
+        eapply start_func; [exact H | clear H]
+    end;
     cbv match beta delta [WeakestPrecondition.func]
   | |- WeakestPrecondition.cmd _ (cmd.set ?s ?e) _ _ _ ?post =>
     unfold1_cmd_goal; cbv beta match delta [cmd_body];
