bedrock2/src/bedrock2/MetricSemantics.v
@@ -1,0 +1,449 @@
+Require Import coqutil.sanity coqutil.Byte.
+Require Import coqutil.Tactics.fwd.
+Require Import coqutil.Map.Properties.
+Require coqutil.Map.SortedListString.
+Require Import bedrock2.Syntax coqutil.Map.Interface coqutil.Map.OfListWord.
+Require Import BinIntDef coqutil.Word.Interface coqutil.Word.Bitwidth.
+Require Export bedrock2.Memory.
+Require Import Coq.Lists.List.
+Require Import bedrock2.MetricLogging.
+Require Import bedrock2.Semantics.
+Require Import Coq.Lists.List.
+
+Section semantics.
+  Context {width: Z} {BW: Bitwidth width} {word: word.word width} {mem: map.map word byte}.
+  Context {locals: map.map String.string word}.
+  Context {ext_spec: ExtSpec}.
+
+  Local Notation metrics := MetricLog.
+
+  Section WithMemAndLocals.
+    Context (m : mem) (l : locals).
+
+    Local Notation "' x <- a | y ; f" := (match a with x => f | _ => y end)
+      (right associativity, at level 70, x pattern).
+
+    Fixpoint eval_expr (e : expr) (mc : metrics) : option (word * metrics) :=
+      match e with
+      | expr.literal v => Some (word.of_Z v, addMetricInstructions 8
+                                             (addMetricLoads 8 mc))
+      | expr.var x => match map.get l x with
+                      | Some v => Some (v, addMetricInstructions 1
+                                           (addMetricLoads 2 mc))
+                      | None => None
+                      end
+      | expr.inlinetable aSize t index =>
+          'Some (index', mc') <- eval_expr index mc | None;
+          'Some v <- load aSize (map.of_list_word t) index' | None;
+          Some (v, (addMetricInstructions 3
+                   (addMetricLoads 4
+                   (addMetricJumps 1 mc'))))
+      | expr.load aSize a =>
+          'Some (a', mc') <- eval_expr a mc | None;
+          'Some v <- load aSize m a' | None;
+          Some (v, addMetricInstructions 1
+                   (addMetricLoads 2 mc'))
+      | expr.op op e1 e2 =>
+          'Some (v1, mc') <- eval_expr e1 mc | None;
+          'Some (v2, mc'') <- eval_expr e2 mc' | None;
+          Some (interp_binop op v1 v2, addMetricInstructions 2
+                                       (addMetricLoads 2 mc''))
+      | expr.ite c e1 e2 =>
+          'Some (vc, mc') <- eval_expr c mc | None;
+          eval_expr (if word.eqb vc (word.of_Z 0) then e2 else e1)
+                    (addMetricInstructions 2
+                       (addMetricLoads 2
+                       (addMetricJumps 1 mc')))
+      end.
+
+    Fixpoint eval_call_args (arges : list expr) (mc : metrics) :=
+      match arges with
+      | e :: tl =>
+        'Some (v, mc') <- eval_expr e mc | None;
+        'Some (args, mc'') <- eval_call_args tl mc' | None;
+        Some (v :: args, mc'')
+      | _ => Some (nil, mc)
+      end.
+
+  End WithMemAndLocals.
+End semantics.
+
+Module exec. Section WithParams.
+  Context {width: Z} {BW: Bitwidth width} {word: word.word width} {mem: map.map word byte}.
+  Context {locals: map.map String.string word}.
+  Context {ext_spec: ExtSpec}.
+  Section WithEnv.
+  Context (e: env).
+
+  Local Notation metrics := MetricLog.
+
+  Implicit Types post : trace -> mem -> locals -> metrics -> Prop. (* COQBUG: unification finds Type instead of Prop and fails to downgrade *)
+  Inductive exec :
+    cmd -> trace -> mem -> locals -> metrics ->
+    (trace -> mem -> locals -> metrics -> Prop) -> Prop :=
+  | skip
+    t m l mc post
+    (_ : post t m l mc)
+    : exec cmd.skip t m l mc post
+  | set x e
+    t m l mc post
+    v mc' (_ : eval_expr m l e mc = Some (v, mc'))
+    (_ : post t m (map.put l x v) (addMetricInstructions 1
+                                  (addMetricLoads 1 mc')))
+    : exec (cmd.set x e) t m l mc post
+  | unset x
+    t m l mc post
+    (_ : post t m (map.remove l x) mc)
+    : exec (cmd.unset x) t m l mc post
+  | store sz ea ev
+    t m l mc post
+    a mc' (_ : eval_expr m l ea mc = Some (a, mc'))
+    v mc'' (_ : eval_expr m l ev mc' = Some (v, mc''))
+    m' (_ : store sz m a v = Some m')
+    (_ : post t m' l (addMetricInstructions 1
+                     (addMetricLoads 1
+                     (addMetricStores 1 mc''))))
+    : exec (cmd.store sz ea ev) t m l mc post
+  | stackalloc x n body
+    t mSmall l mc post
+    (_ : Z.modulo n (bytes_per_word width) = 0)
+    (_ : forall a mStack mCombined,
+        anybytes a n mStack ->
+        map.split mCombined mSmall mStack ->
+        exec body t mCombined (map.put l x a) (addMetricInstructions 1 (addMetricLoads 1 mc))
+          (fun t' mCombined' l' mc' =>
+            exists mSmall' mStack',
+              anybytes a n mStack' /\
+              map.split mCombined' mSmall' mStack' /\
+              post t' mSmall' l' mc'))
+     : exec (cmd.stackalloc x n body) t mSmall l mc post
+  | if_true t m l mc e c1 c2 post
+    v mc' (_ : eval_expr m l e mc = Some (v, mc'))
+    (_ : word.unsigned v <> 0)
+    (_ : exec c1 t m l (addMetricInstructions 2
+                       (addMetricLoads 2
+                       (addMetricJumps 1 mc'))) post)
+    : exec (cmd.cond e c1 c2) t m l mc post
+  | if_false e c1 c2
+    t m l mc post
+    v mc' (_ : eval_expr m l e mc = Some (v, mc'))
+    (_ : word.unsigned v = 0)
+    (_ : exec c2 t m l (addMetricInstructions 2
+                       (addMetricLoads 2
+                       (addMetricJumps 1 mc'))) post)
+    : exec (cmd.cond e c1 c2) t m l mc post
+  | seq c1 c2
+    t m l mc post
+    mid (_ : exec c1 t m l mc mid)
+    (_ : forall t' m' l' mc', mid t' m' l' mc' -> exec c2 t' m' l' mc' post)
+    : exec (cmd.seq c1 c2) t m l mc post
+  | while_false e c
+    t m l mc post
+    v mc' (_ : eval_expr m l e mc = Some (v, mc'))
+    (_ : word.unsigned v = 0)
+    (_ : post t m l (addMetricInstructions 1
+                    (addMetricLoads 1
+                    (addMetricJumps 1 mc'))))
+    : exec (cmd.while e c) t m l mc post
+  | while_true e c
+      t m l mc post
+      v mc' (_ : eval_expr m l e mc = Some (v, mc'))
+      (_ : word.unsigned v <> 0)
+      mid (_ : exec c t m l mc' mid)
+      (_ : forall t' m' l' mc'', mid t' m' l' mc'' ->
+                                 exec (cmd.while e c) t' m' l' (addMetricInstructions 2
+                                                               (addMetricLoads 2
+                                                               (addMetricJumps 1 mc''))) post)
+    : exec (cmd.while e c) t m l mc post
+  | call binds fname arges
+      t m l mc post
+      params rets fbody (_ : map.get e fname = Some (params, rets, fbody))
+      args mc' (_ : eval_call_args m l arges mc = Some (args, mc'))
+      lf (_ : map.of_list_zip params args = Some lf)
+      mid (_ : exec fbody t m lf (addMetricInstructions 100 (addMetricJumps 100 (addMetricLoads 100 (addMetricStores 100 mc')))) mid)
+      (_ : forall t' m' st1 mc'', mid t' m' st1 mc'' ->
+          exists retvs, map.getmany_of_list st1 rets = Some retvs /\
+          exists l', map.putmany_of_list_zip binds retvs l = Some l' /\
+          post t' m' l'  (addMetricInstructions 100 (addMetricJumps 100 (addMetricLoads 100 (addMetricStores 100 mc'')))))
+    : exec (cmd.call binds fname arges) t m l mc post
+  | interact binds action arges
+      t m l mc post
+      mKeep mGive (_: map.split m mKeep mGive)
+      args mc' (_ :  eval_call_args m l arges mc = Some (args, mc'))
+      mid (_ : ext_spec t mGive action args mid)
+      (_ : forall mReceive resvals, mid mReceive resvals ->
+          exists l', map.putmany_of_list_zip binds resvals l = Some l' /\
+          forall m', map.split m' mKeep mReceive ->
+          post (cons ((mGive, action, args), (mReceive, resvals)) t) m' l'
+            (addMetricInstructions 1
+            (addMetricStores 1
+            (addMetricLoads 2 mc'))))
+    : exec (cmd.interact binds action arges) t m l mc post
+  .
+
+  Context {word_ok: word.ok word} {mem_ok: map.ok mem} {ext_spec_ok: ext_spec.ok ext_spec}.
+
+  Lemma weaken: forall t l m mc s post1,
+      exec s t m l mc post1 ->
+      forall post2: _ -> _ -> _ -> _ -> Prop,
+        (forall t' m' l' mc', post1 t' m' l' mc' -> post2 t' m' l' mc') ->
+        exec s t m l mc post2.
+  Proof.
+    induction 1; intros; try solve [econstructor; eauto].
+    - eapply stackalloc. 1: assumption.
+      intros.
+      eapply H1; eauto.
+      intros. fwd. eauto 10.
+    - eapply call.
+      4: eapply IHexec.
+      all: eauto.
+      intros.
+      edestruct H3 as (? & ? & ? & ? & ?); [eassumption|].
+      eauto 10.
+    - eapply interact; try eassumption.
+      intros.
+      edestruct H2 as (? & ? & ?); [eassumption|].
+      eauto 10.
+  Qed.
+
+  Lemma intersect: forall t l m mc s post1,
+      exec s t m l mc post1 ->
+      forall post2,
+        exec s t m l mc post2 ->
+        exec s t m l mc (fun t' m' l' mc' => post1 t' m' l' mc' /\ post2 t' m' l' mc').
+  Proof.
+    induction 1;
+      intros;
+      match goal with
+      | H: exec _ _ _ _ _ _ |- _ => inversion H; subst; clear H
+      end;
+      try match goal with
+      | H1: ?e = Some (?x1, ?y1, ?z1), H2: ?e = Some (?x2, ?y2, ?z2) |- _ =>
+        replace x2 with x1 in * by congruence;
+          replace y2 with y1 in * by congruence;
+          replace z2 with z1 in * by congruence;
+          clear x2 y2 z2 H2
+      end;
+      repeat match goal with
+             | H1: ?e = Some (?v1, ?mc1), H2: ?e = Some (?v2, ?mc2) |- _ =>
+               replace v2 with v1 in * by congruence;
+               replace mc2 with mc1 in * by congruence; clear H2
+             end;
+      repeat match goal with
+             | H1: ?e = Some ?v1, H2: ?e = Some ?v2 |- _ =>
+               replace v2 with v1 in * by congruence; clear H2
+             end;
+      try solve [econstructor; eauto | exfalso; congruence].
+
+    - econstructor. 1: eassumption.
+      intros.
+      rename H0 into Ex1, H12 into Ex2.
+      eapply weaken. 1: eapply H1. 1,2: eassumption.
+      1: eapply Ex2. 1,2: eassumption.
+      cbv beta.
+      intros. fwd.
+      lazymatch goal with
+      | A: map.split _ _ _, B: map.split _ _ _ |- _ =>
+        specialize @map.split_diff with (4 := A) (5 := B) as P
+      end.
+      edestruct P; try typeclasses eauto. 2: subst; eauto 10.
+      eapply anybytes_unique_domain; eassumption.
+    - econstructor.
+      + eapply IHexec. exact H5. (* not H *)
+      + simpl. intros *. intros [? ?]. eauto.
+    - eapply while_true. 1, 2: eassumption.
+      + eapply IHexec. exact H9. (* not H1 *)
+      + simpl. intros *. intros [? ?]. eauto.
+    - eapply call. 1, 2, 3: eassumption.
+      + eapply IHexec. exact H16. (* not H2 *)
+      + simpl. intros *. intros [? ?].
+        edestruct H3 as (? & ? & ? & ? & ?); [eassumption|].
+        edestruct H17 as (? & ? & ? & ? & ?); [eassumption|].
+        repeat match goal with
+               | H1: ?e = Some ?v1, H2: ?e = Some ?v2 |- _ =>
+                 replace v2 with v1 in * by congruence; clear H2
+               end.
+        eauto 10.
+    - pose proof ext_spec.unique_mGive_footprint as P.
+      specialize P with (1 := H1) (2 := H14).
+      destruct (map.split_diff P H H7). subst mKeep0 mGive0. clear H7.
+      eapply interact. 1,2: eassumption.
+      + eapply ext_spec.intersect; [ exact H1 | exact H14 ].
+      + simpl. intros *. intros [? ?].
+        edestruct H2 as (? & ? & ?); [eassumption|].
+        edestruct H15 as (? & ? & ?); [eassumption|].
+        repeat match goal with
+               | H1: ?e = Some ?v1, H2: ?e = Some ?v2 |- _ =>
+                 replace v2 with v1 in * by congruence; clear H2
+               end.
+        eauto 10.
+  Qed.
+
+  End WithEnv.
+
+  Lemma extend_env: forall e1 e2,
+      map.extends e2 e1 ->
+      forall c t m l mc post,
+      exec e1 c t m l mc post ->
+      exec e2 c t m l mc post.
+  Proof. induction 2; try solve [econstructor; eauto]. Qed.
+
+  End WithParams.
+End exec. Notation exec := exec.exec.
+
+Section WithParams.
+  Context {width: Z} {BW: Bitwidth width} {word: word.word width} {mem: map.map word byte}.
+  Context {locals: map.map String.string word}.
+  Context {ext_spec: ExtSpec}.
+
+  Implicit Types (l: locals) (m: mem).
+
+  Definition call e fname t m args mc post :=
+    exists argnames retnames body,
+      map.get e fname = Some (argnames, retnames, body) /\
+      exists l, map.of_list_zip argnames args = Some l /\
+        exec e body t m l mc (fun t' m' l' mc' => exists rets,
+          map.getmany_of_list l' retnames = Some rets /\ post t' m' rets mc').
+
+  Lemma weaken_call: forall e fname t m args mc post1,
+      call e fname t m args mc post1 ->
+      forall (post2: trace -> mem -> list word -> MetricLog -> Prop),
+      (forall t' m' rets mc', post1 t' m' rets mc' -> post2 t' m' rets mc') ->
+      call e fname t m args mc post2.
+  Proof.
+    unfold call. intros. fwd.
+    do 4 eexists. 1: eassumption.
+    do 2 eexists. 1: eassumption.
+    eapply exec.weaken. 1: eassumption.
+    cbv beta. clear -H0. intros. fwd. eauto.
+  Qed.
+
+  Lemma extend_env_call: forall e1 e2,
+      map.extends e2 e1 ->
+      forall f t m rets mc post,
+      call e1 f t m rets mc post ->
+      call e2 f t m rets mc post.
+  Proof.
+    unfold call. intros. fwd. repeat eexists.
+    - eapply H. eassumption.
+    - eassumption.
+    - eapply exec.extend_env; eassumption.
+  Qed.
+
+  Lemma of_metrics_free_eval_expr: forall m l e v,
+      Semantics.eval_expr m l e = Some v ->
+      forall mc, exists mc', MetricSemantics.eval_expr m l e mc = Some (v, mc').
+  Proof.
+    induction e; cbn; intros;
+      repeat match goal with
+        | H: Some _ = Some _ |- _ => eapply Option.eq_of_eq_Some in H; subst
+        | H: _ = Some _ |- _ => rewrite H
+        | IH: forall _, Some _ = Some _ -> _ |- _ => specialize IH with (1 := eq_refl)
+        | IH: forall _: MetricLog, exists _: MetricLog, eval_expr ?m ?l ?e _ = Some _
+          |- context[eval_expr ?m ?l ?e ?mc] => specialize (IH mc)
+        | |- _ => progress fwd
+        | |- _ => Tactics.destruct_one_match
+        end;
+      eauto.
+  Qed.
+
+  Lemma to_metrics_free_eval_expr: forall m l e mc v mc',
+      MetricSemantics.eval_expr m l e mc = Some (v, mc') ->
+      Semantics.eval_expr m l e = Some v.
+  Proof.
+    induction e; cbn; intros; fwd;
+      repeat match goal with
+        | IH: forall _ _ _, eval_expr _ _ _ _ = _ -> _, H: eval_expr _ _ _ _ = _ |- _ =>
+          specialize IH with (1 := H)
+        | H: _ = Some _ |- _ => rewrite H
+        | |- _ => Tactics.destruct_one_match
+        end;
+    try congruence.
+  Qed.
+
+  Lemma of_metrics_free_eval_call_args: forall m l arges args,
+      Semantics.eval_call_args m l arges = Some args ->
+      forall mc, exists mc', MetricSemantics.eval_call_args m l arges mc = Some (args, mc').
+  Proof.
+    induction arges; cbn; intros.
+    - eapply Option.eq_of_eq_Some in H. subst. eauto.
+    - fwd.
+      eapply of_metrics_free_eval_expr in E. destruct E as (mc' & E). rewrite E.
+      specialize IHarges with (1 := eq_refl). specialize (IHarges mc').
+      destruct IHarges as (mc'' & IH). rewrite IH. eauto.
+  Qed.
+
+  Lemma to_metrics_free_eval_call_args: forall m l arges mc args mc',
+      MetricSemantics.eval_call_args m l arges mc = Some (args, mc') ->
+      Semantics.eval_call_args m l arges = Some args.
+  Proof.
+    induction arges; cbn; intros.
+    - congruence.
+    - fwd.
+      eapply to_metrics_free_eval_expr in E. rewrite E.
+      specialize IHarges with (1 := E0). rewrite IHarges. reflexivity.
+  Qed.
+
+  Context (e: env).
+
+  Lemma of_metrics_free: forall c t m l post,
+      Semantics.exec e c t m l post ->
+      forall mc, MetricSemantics.exec e c t m l mc (fun t' m' l' _ => post t' m' l').
+  Proof.
+    induction 1; intros;
+      repeat match reverse goal with
+        | H: Semantics.eval_expr _ _ _ = Some _ |- _ =>
+            eapply of_metrics_free_eval_expr in H; destruct H as (? & H)
+        | H: Semantics.eval_call_args _ _ _ = Some _ |- _ =>
+            eapply of_metrics_free_eval_call_args in H; destruct H as (? & H)
+        end;
+      try solve [econstructor; eauto].
+  Qed.
+
+  Lemma to_metrics_free: forall c t m l mc post,
+      MetricSemantics.exec e c t m l mc post ->
+      Semantics.exec e c t m l (fun t' m' l' => exists mc', post t' m' l' mc').
+  Proof.
+    induction 1; intros;
+      repeat match reverse goal with
+        | H: eval_expr _ _ _ _ = Some _ |- _ =>
+            eapply to_metrics_free_eval_expr in H
+        | H: eval_call_args _ _ _ _ = Some _ |- _ =>
+            eapply to_metrics_free_eval_call_args in H
+        end;
+      try solve [econstructor; eauto].
+    { econstructor. 1: eauto.
+      intros.
+      eapply Semantics.exec.weaken. 1: eapply H1. all: eauto.
+      cbv beta.
+      clear. firstorder idtac. }
+    { econstructor.
+      1: eapply IHexec.
+      cbv beta. intros.
+      fwd.
+      eapply H1. eassumption. }
+    { econstructor; [ eassumption .. | ].
+      cbv beta. intros. fwd. eapply H3. eassumption. }
+    { econstructor. 1-4: eassumption.
+      cbv beta. intros. fwd. specialize H3 with (1 := H4). fwd. eauto 10. }
+    { econstructor. 1-3: eassumption.
+      intros. specialize H2 with (1 := H3). fwd. eauto. }
+  Qed.
+
+  Lemma of_metrics_free_call: forall f t m args post,
+      Semantics.call e f t m args post ->
+      forall mc, call e f t m args mc (fun t' m' rets _ => post t' m' rets).
+  Proof.
+    unfold call, Semantics.call. intros. fwd. eauto 10 using of_metrics_free.
+  Qed.
+
+  Lemma to_metrics_free_call: forall f t m args mc post,
+      call e f t m args mc post ->
+      Semantics.call e f t m args (fun t' m' rets => exists mc', post t' m' rets mc').
+  Proof.
+    unfold call, Semantics.call. intros. fwd.
+    do 4 eexists. 1: eassumption. do 2 eexists. 1: eassumption.
+    eapply Semantics.exec.weaken. 1: eapply to_metrics_free. 1: eassumption.
+    cbv beta. clear. firstorder idtac.
+  Qed.
+End WithParams.
