bedrock2/src/bedrock2/Refinement.v
@@ -1,0 +1,46 @@
+(* These lemmas can be useful when proving a refinement and induction over the
+   statement rather than over its exec derivation is preferred *)
+
+Require Import Coq.ZArith.ZArith.
+Require Import coqutil.Word.Bitwidth.
+Require Import coqutil.Map.Interface.
+Require Import bedrock2.Syntax bedrock2.Semantics.
+
+Section WithParams.
+  Context {width: Z} {BW: Bitwidth width} {word: word.word width}.
+  Context {mem: map.map word Byte.byte}.
+  Context {locals: map.map String.string word}.
+  Context {ext_spec: bedrock2.Semantics.ExtSpec}.
+
+  Definition refines(c2 c1: cmd) := forall functions t m l post,
+      Semantics.exec.exec functions c1 t m l post ->
+      Semantics.exec.exec functions c2 t m l post.
+
+  Lemma refinement_while: forall test body1 body2,
+      refines body2 body1 ->
+      refines (cmd.while test body2) (cmd.while test body1).
+  Proof.
+    unfold refines. intros * R *.
+    remember (cmd.while test body1) as c1. intros. revert Heqc1.
+    induction H; intros; subst; inversion Heqc1; subst.
+    - eapply Semantics.exec.while_false; eassumption.
+    - eapply Semantics.exec.while_true; try eassumption.
+      { unfold refines in R.
+        eapply R. eassumption. }
+      intros.
+      eapply H3; eauto.
+  Qed.
+
+  Lemma refinement_seq: forall c1 c2 c1' c2',
+      refines c1' c1 ->
+      refines c2' c2 ->
+      refines (cmd.seq c1' c2') (cmd.seq c1 c2).
+  Proof.
+    intros * R1 R2 functions t m l post H.
+    unfold refines in *.
+    inversion H. subst. clear H.
+    eapply Semantics.exec.seq.
+    - eapply R1. eassumption.
+    - intros * Hmid. eapply R2. eauto.
+  Qed.
+End WithParams.
