bedrock2/src/bedrock2Examples/SPI.v
@@ -130,6 +130,17 @@ Section WithParameters.
       cbv [isMMIOAddr addr].
       ZnWords. }
     repeat straightline.
+    (* The hnf inside this letexists used to substitute
+
+         c := cmd.cond (expr.op bopname.sru "busy" 31) cmd.skip
+                (cmd.set "i" (expr.op bopname.xor "i" "i")) : cmd.cmd
+
+       and also unfolded WeakestPrecondition.cmd of c into
+
+         WeakestPrecondition.dexpr m l0 cond letboundEvar /\
+         ThenCorrectness /\
+         ElseCorrectness
+    *)
     letexists. split.
     { repeat straightline. }
     split; intros.
