compiler/src/compiler/ExprImpEventLoopSpec.v
@@ -2,6 +2,7 @@ Require Import Coq.ZArith.ZArith.
 Require Coq.Strings.String.
 Require Import coqutil.Map.Interface coqutil.Word.Interface.
 Require Import bedrock2.MetricLogging.
+Require Import bedrock2.Semantics.
 Require Import compiler.SeparationLogic.
 Require Import compiler.LowerPipeline.
 Require Import compiler.Pipeline.
@@ -9,7 +10,6 @@ Require Import compiler.Pipeline.
 Section Params1.
   Context {width} {BW: Bitwidth width} {word: word.word width} {mem: map.map word Byte.byte}.
   Context {locals: map.map String.string word}.
-  Context {env: map.map String.string (list String.string * list String.string * Syntax.cmd)}.
   Context {ext_spec: Semantics.ExtSpec}.
 
   Set Implicit Arguments.
@@ -37,15 +37,15 @@ Section Params1.
   {
     funs_valid: valid_src_funs e = true;
     init_code: Syntax.cmd.cmd;
-    get_init_code: map.get (map.of_list e) init_f = Some (nil, nil, init_code);
+    get_init_code: map.get (map.of_list e : env) init_f = Some (nil, nil, init_code);
     init_code_correct: forall m0 mc0,
         mem_available spec.(datamem_start) spec.(datamem_pastend) m0 ->
-        Semantics.exec (map.of_list e) init_code nil m0 map.empty mc0 (hl_inv spec);
+        MetricSemantics.exec (map.of_list e) init_code nil m0 map.empty mc0 (hl_inv spec);
     loop_body: Syntax.cmd.cmd;
-    get_loop_body: map.get (map.of_list e) loop_f = Some (nil, nil, loop_body);
+    get_loop_body: map.get (map.of_list e : env) loop_f = Some (nil, nil, loop_body);
     loop_body_correct: forall t m l mc,
         hl_inv spec t m l mc ->
-        Semantics.exec (map.of_list e) loop_body t m l mc (hl_inv spec);
+        MetricSemantics.exec (map.of_list e) loop_body t m l mc (hl_inv spec);
   }.
 
 End Params1.
